TMR memcmp proof done

Examples/tmr/tmr_ft_proof.v
@@ -510,3 +510,536 @@ Proof.
       apply Answer2 in H. contradiction.
       apply Answer1 in H. contradiction.
 Qed.
+
+Section FaultTolerantInvariants.
+    Variable mem : memory.
+    Variable raddr : addr.
+    Variable in_a in_b : addr.
+    Variable len : N.
+    Variable s0 s1 s2 s3 s4 sp : N.
+
+    (* When running CRYPTO_memcmp, there are three distinct possibilities:
+        1. s FC = 0, no fault occurs, s' FC = 0
+        2. s FC = 1, no fault occurs, s' FC = 1
+        3. s FC = 1,  a fault occurs, s' FC = 0
+
+        When running passwords_match_tmr, after each call, these cases must
+        each be analyzed. I predict this will hurt automation.
+    *)
+
+    (* These values are always preserved because CRYPTO_memcmp
+       never touches them *)
+    Definition safe_regs (s : store) :=
+        s R_RA = raddr /\
+        s R_S0 = s0 /\ s R_S1 = s1 /\ s R_S2 = s2 /\
+        s R_S3 = s3 /\ s R_S4 = s4 /\
+        s R_SP = sp /\
+        s V_MEM32 = mem.
+
+    Definition ft_invs T (Inv Post: inv_type T) (NoInv:T) (s:store) (a:addr) : T :=
+        let postcondition := postcondition mem in_a in_b len in
+        let noverlaps := noverlaps in_a in_b len in
+        let stack := stack mem raddr s0 s1 s2 s3 s4 sp in
+        match a with
+        (* CRYPTO_memcmp *)
+        | 0x10170 => Inv 0
+            (s V_FC <= 1 /\
+             s R_A0 = in_a /\ s R_A1 = in_b /\ s R_A2 = len /\
+             safe_regs s)
+        | 0x10180 => Inv 0
+            (safe_regs s /\
+             (* Cases 1, 2 *)
+             ((s V_FC <= 1 /\ exists k,
+              s V_MEM32 = mem /\
+              s R_A5 = in_a ⊕ k /\
+              s R_A1 = in_b ⊕ k /\
+              s R_A2 = in_a ⊕ len /\
+              k < len < 2^32 /\
+              ((s R_A0 = 0) <-> k_equal in_a in_b k mem) /\
+              safe_regs s) \/
+             (* Case 3 *)
+              s V_FC = 0)
+            )
+        | 0x1019c | 0x101a4 => Post 0 
+            (safe_regs s /\
+             (* Cases 1, 2 *)
+             ((s V_FC <= 1 /\ postcondition s None None) \/
+             (* Case 3 *)
+             s V_FC = 0))
+
+        (* passwords_match_tmr *)
+        | 0x101a8 => Inv 1
+            (s R_A0 = in_a /\ s R_A1 = in_b /\ s R_A2 = len /\
+             safe_regs s /\ noverlaps (s R_SP) /\
+             s V_FC = 1)
+        | 0x101f4 => Inv 1
+            (s R_A0 = in_a /\ s R_A1 = in_b /\ s R_A2 = len /\
+             s R_S0 = in_a /\ s R_S1 = in_b /\ s R_S2 = len /\
+             noverlaps (s R_SP ⊕ ssize) /\ stack s /\
+             s V_FC <= 1)
+        | 0x10208 => Inv 1
+            (safe_regs s /\ noverlaps (s R_SP ⊕ ssize) /\
+             (* Cases 1, 2 *)
+             ((s V_FC <= 1 /\
+               s R_A0 = in_a /\ s R_A1 = in_b /\ s R_A2 = len /\
+               s R_S0 = in_a /\ s R_S1 = in_b /\ s R_S2 = len /\
+               postcondition s (Some R_S3) (Some (s V_MEM32))) \/
+               (* Case 3 *)
+               s V_FC = 0))
+        | 0x1021c => Inv 1
+            (s R_A0 = in_a /\ s R_A1 = in_b /\ s R_A2 = len /\ 
+             s R_S0 = in_a /\ s R_S1 = in_b /\ s R_S2 = len /\
+             postcondition s (Some R_S4) (Some (s V_MEM32)) /\
+             postcondition s (Some R_S3) (Some (s V_MEM32)) /\
+             noverlaps (s R_SP ⊕ ssize) /\
+             stack s)
+        | 0x10220 => Inv 1
+            (postcondition s (Some R_S4) (Some (s V_MEM32)) /\
+             postcondition s (Some R_S3) (Some (s V_MEM32)) /\
+             postcondition s None (Some (s V_MEM32)) /\
+             stack s)
+        | 0x102b0 | 0x102b4 => Post 1 (
+            s R_A0 = 1 <-> k_equal in_a in_b len (s V_MEM32)
+        )
+        | _ => NoInv
+        end.
+
+    Definition tmr_fault : program := inject_fault tmr_ft.
+
+    Definition ft_exits0 := make_exits 0 tmr_fault ft_invs.
+    Definition ft_invs0 := make_invs 0 tmr_fault ft_invs.
+
+    Definition ft_exits1 := make_exits 1 tmr_fault ft_invs.
+    Definition ft_invs1 := make_invs 1 tmr_fault ft_invs.
+End FaultTolerantInvariants.
+
+(* Proof in fault-aware context *)
+Theorem crypto_memcmp_correctness_ft:
+  forall s mem t xs' in_a in_b len raddr s0 s1 s2 s3 s4 sp
+         (ENTRY: startof t xs' = (Addr 0x10170, s))
+         (MDL: models rvtypctx s)
+         (MEM: s V_MEM32 = mem)
+         (A0: s R_A0 = in_a)
+         (A1: s R_A1 = in_b)
+         (LEN: s R_A2 = len)
+         (RA: s R_RA = raddr)
+         (S0: s R_S0 = s0)
+         (S1: s R_S1 = s1)
+         (S2: s R_S2 = s2)
+         (S3: s R_S3 = s3)
+         (S4: s R_S4 = s4)
+         (SP: s R_SP = sp)
+         (FC: s V_FC <= 1),
+  satisfies_all tmr_fault 
+                       (ft_invs0 mem raddr in_a in_b len s0 s1 s2 s3 s4 sp)
+                       (ft_exits0 mem raddr in_a in_b len s0 s1 s2 s3 s4 sp)
+                       (xs'::t).
+Proof using.
+    Local Ltac step ::= 
+        match goal with
+        | [s' : store, FC : ?s' V_FC <= 1 |- _] =>
+            let H := fresh "H" in
+            assert (s' V_FC = 0 \/ s' V_FC = 1) as H by lia;
+            clear FC; destruct H
+        | _ => idtac
+        end;
+        time r5_step;
+        repeat match goal with
+        | [n : N, BC : ?n mod 2 = _ |- _] => clear BC n
+        | [s' : store, n : N, 
+            BC : (if 0 <? ?s' V_FC then ?n mod 2 else 0) = _ |- _] => clear BC n
+        | [H: ?x = ?x |- _] => clear H
+        end;
+        try discriminate.
+    intros. apply prove_invs.
+
+    simpl. rewrite ENTRY. step; repeat split; auto; lia. 
+
+    intros.
+    eapply startof_prefix in ENTRY; try eassumption.
+    eapply preservation_exec_prog in MDL; try (eassumption || apply inject_fault_lift_riscv_welltyped).
+    clear - PRE MDL. rename t1 into t. rename s5 into s. rename a1 into a.
+
+    destruct_inv 32 PRE.
+
+    (* Intro *)
+    destruct PRE as (FC & A0 & A1 & A2 & Safe). {
+    Local Ltac solve_inv MDL A2 :=
+        exists 0; psimpl; repeat split; auto;
+            [lia|
+            apply (models_var R_A2) in MDL; rewrite <- A2; apply MDL
+            |lia|unfold k_equal; lia].
+    step.
+    - (* len = 0, fault *)
+        repeat step; split;
+        [unfold safe_regs in *; now psimpl
+        |left; split; [lia|]];
+        unfold postcondition; psimpl;
+            unfold k_equal; split; lia.
+    - (* len <> 0, fault *)
+        repeat step; split;
+        [unfold safe_regs in *; now psimpl
+        |left; split; [lia|]];
+        exists 0; psimpl; unfold safe_regs in Safe;
+        repeat split; try solve [intuition];
+        unfold k_equal; try lia;
+        apply (models_var R_A2) in MDL; simpl in MDL; lia.
+    - (* no fault *) 
+        repeat step;
+            (split; 
+            [unfold safe_regs in *; now psimpl
+            |solve [now right]||left]);
+            split; [reflexivity|];
+            unfold postcondition; psimpl;
+            split; intro; unfold k_equal; lia.
+    - (* no fault *) 
+        repeat step;
+            (split; 
+            [unfold safe_regs in *; now psimpl
+            |solve [now right]||left]);
+            split; [reflexivity|];
+            exists 0; psimpl; unfold safe_regs in *;
+            repeat split; try solve [intuition];
+            unfold k_equal; try lia;
+            apply (models_var R_A2) in MDL; simpl in MDL; lia.
+    - (* no fault *) 
+        repeat step;
+            (split; 
+            [unfold safe_regs in *; now psimpl
+            |solve [now right]||left]).
+    }
+
+    (* Loop *)
+    destruct PRE as (Safe & [PRE|PRE]).
+    destruct PRE as (FC & k & Mem & A5 & A1 & A2 & Bound & Eq). {
+    Local Ltac solve_inv' k Eq :=
+        let X := fresh "X" in
+        let Y := fresh "Y" in
+        let Z := fresh "Z" in
+        let W := fresh "W" in
+        let Inv := fresh "Inv" in
+        let i := fresh "i" in
+        exists (k ⊕ 1); psimpl; unfold safe_regs in *; psimpl;
+        repeat split; try solve [intuition];
+        [lia
+        |unfold k_equal; intros X i Z; apply or_xor_zero in X; destruct X;
+            assert (i < k \/ i = k) as Y by lia; destruct Y;
+            [now apply Eq|now subst]
+        |repeat split; intros W; rewrite N.mod_small in W by lia;
+            pose proof (k_equal_inv _ _ _ _ W) as Inv; apply Eq in Inv;
+            specialize (W k ltac:(lia));
+            now rewrite W, N.lxor_nilpotent, Inv].
+    Local Ltac solve_post k len s Eq :=
+        let X := fresh "H" in
+        let i := fresh "i" in
+        let ILen := fresh "ilen" in
+        let KLen := fresh "klen" in
+        assert (1 + k = len) as KLen by lia;
+        subst len;
+        split; intro X;
+            [apply k_equal_step;
+              apply or_xor_zero in X; destruct X;
+              [apply Eq; assumption|now symmetry]
+            |replace (s R_A0) with 0; psimpl;
+              [apply N.lxor_eq_0_iff; symmetry; apply X; lia
+              |apply k_equal_inv in X; symmetry; apply Eq, X]
+            ].
+    repeat step;
+        (split; 
+         [unfold safe_regs in *; now psimpl
+         |(now right) || (left; split; [lia|])]).
+        solve_inv' k Eq.
+        solve_post k len s Eq.
+    }
+
+    repeat step; (split;
+        [unfold safe_regs in *; now psimpl
+        |now right]).
+Qed.
+
+(* Proof in fault-free environment *)
+Theorem tmr_ft_correctness:
+  forall s mem t xs' in_a in_b len raddr s0 s1 s2 s3 s4 sp
+         (ENTRY: startof t xs' = (Addr 0x101a8, s))
+         (MDL: models rvtypctx s)
+         (MEM: s V_MEM32 = mem)
+         (A0: s R_A0 = in_a)
+         (A1: s R_A1 = in_b)
+         (LEN: s R_A2 = len)
+         (RA: s R_RA = raddr)
+         (S0: s R_S0 = s0)
+         (S1: s R_S1 = s1)
+         (S2: s R_S2 = s2)
+         (S3: s R_S3 = s3)
+         (S4: s R_S4 = s4)
+         (SP: s R_SP = sp)
+         (NVL: noverlaps in_a in_b len sp),
+  satisfies_all tmr_ft (invs1 mem raddr in_a in_b len s0 s1 s2 s3 s4 sp)
+                       (exits1 mem raddr in_a in_b len s0 s1 s2 s3 s4 sp) (xs'::t).
+Proof.
+    intros. apply prove_invs.
+
+    simpl. rewrite ENTRY. step. rewrite SP.
+    repeat (split; auto).
+
+    intros.
+    eapply startof_prefix in ENTRY; try eassumption.
+    eapply preservation_exec_prog in MDL; try (eassumption || apply lift_riscv_welltyped).
+    clear - PRE MDL. rename t1 into t. rename s5 into s. rename a1 into a.
+
+    destruct_inv 32 PRE.
+
+    Ltac riscv_call thm :=
+        let MDL1 := fresh "MDL1" in
+        let s1 := fresh "s1" in
+        set (s1 := update _ _ _);
+        eapply models_after_steps;
+        [assumption|apply lift_riscv_welltyped|];
+        intro MDL1; eapply (perform_call 0);
+        [reflexivity|intros;
+                     eapply thm; 
+                     try reflexivity; eauto|reflexivity|];
+        let a := fresh "a" in
+        let s' := fresh "s'" in
+        let t2 := fresh "t2" in
+        intros
+            a' s' t2 ENTRY XP UT PRE
+        ; unfold s1 in PRE; psimpl in PRE;
+        let MDL' := fresh "MDL'" in
+        assert (models rvtypctx s') as MDL' by
+            (eapply preservation_exec_prog;
+             eauto using lift_riscv_welltyped);
+        unfold archtyps in *;
+        match goal with
+        | [|- context[?t2 ++ ?t0 ++ (Addr ?x, ?s) :: ?t]] =>
+            let t' := fresh "t'" in
+            set (t' := t2++t0++(Addr x, s)::t) in *; clearbody s1;
+            let MDL := fresh "MDL" in
+            rename MDL' into MDL;
+            destruct_inv 32 PRE
+        end.
+
+    (* Intro *)
+    destruct PRE as (A0 & A1 & A2 & S0 & S1 & S2 & S3 & S4 & SP & RA & Mem & NVL). {
+    do 20 step.
+
+    (* Dummy hyp to make it easier to use the above tactic *)
+    eassert (ST: stack mem raddr s0 s1 s2 s3 s4 sp 
+        (update s V_MEM32 _)).
+        unfold stack; now psimpl.
+
+    (* Call CRYPTO_memcmp *)
+    riscv_call crypto_memcmp_correctness;
+        (destruct PRE as (Answer1 & RA' & S0' & S1' & S2' & S3' & S4' & SP' & Mem');
+        unfold postcondition in Answer1; repeat step;
+        repeat (split; [reflexivity|]); split; [
+            unfold postcondition; split; intro; [
+                apply Answer1 in H; intros a ALen;
+                specialize (H a ALen);
+                repeat (rewrite getmem_noverlap in H; [|
+                    ((apply (noverlap_shrink _ in_a len);
+                        [psimpl; lia|]) ||
+                    (apply (noverlap_shrink _ in_b len);
+                        [psimpl; lia|]));
+                    apply noverlap_symmetry,
+                        (noverlap_shrink _ (s5 R_SP ⊖ 32) 32);
+                        [psimpl; lia|];
+                    apply noverlap_symmetry; now destruct NVL]);
+                rewrite Mem';
+                now repeat (rewrite getmem_noverlap; [|
+                    ((apply (noverlap_shrink _ in_a len);
+                        [psimpl; lia|]) ||
+                    (apply (noverlap_shrink _ in_b len);
+                        [psimpl; lia|]));
+                    apply noverlap_symmetry,
+                        (noverlap_shrink _ (s5 R_SP ⊖ 32) 32);
+                        [psimpl; lia|];
+                    apply noverlap_symmetry; now destruct NVL])
+            | psimpl; apply Answer1; intros a ALen;
+                specialize (H a ALen);
+                rewrite Mem' in H;
+                repeat (rewrite getmem_noverlap in H; [|
+                    ((apply (noverlap_shrink _ in_a len);
+                        [psimpl; lia|]) ||
+                    (apply (noverlap_shrink _ in_b len);
+                        [psimpl; lia|]));
+                    apply noverlap_symmetry,
+                        (noverlap_shrink _ (s5 R_SP ⊖ 32) 32);
+                        [psimpl; lia|];
+                    apply noverlap_symmetry; now destruct NVL
+                ]);
+                now repeat (rewrite getmem_noverlap; [|
+                    ((apply (noverlap_shrink _ in_a len);
+                        [psimpl; lia|]) ||
+                    (apply (noverlap_shrink _ in_b len);
+                        [psimpl; lia|]));
+                    apply noverlap_symmetry,
+                        (noverlap_shrink _ (s5 R_SP ⊖ 32) 32);
+                        [psimpl; lia|];
+                    apply noverlap_symmetry; now destruct NVL])]
+        |]; split; [unfold noverlaps in *; psimpl; 
+            now rewrite SP', <- SP
+        |unfold stack; psimpl; now rewrite Mem']).
+    }
+
+    (* To second call *)
+    destruct PRE as (A0 & A1 & A2 & S0 & S1 & S2 & Answer1 & NVL & ST). {
+    step.
+
+    (* Formal goal for riscv_call*)
+    match goal with
+    | [|- context[?x :: ?y :: ?t]] =>
+        change (x :: y :: t) with
+            (x :: nil ++ y :: t)
+    end.
+
+    (* Call CRYPTO_memcmp *)
+    riscv_call crypto_memcmp_correctness;
+        (destruct PRE as (Answer2 & RA & S0' & S1' & S2' & S3 & S4 & SP & MEM);
+        unfold postcondition in Answer2; repeat step;
+        repeat (split; [solve[reflexivity||auto]|]); split; [
+            unfold postcondition; split; intro; [
+                apply Answer2 in H; intros a ALen;
+                rewrite A2 in H;
+                specialize (H a ALen);
+                repeat (rewrite getmem_noverlap in H; [|
+                    ((apply (noverlap_shrink _ in_a len);
+                        [psimpl; lia|]) ||
+                    (apply (noverlap_shrink _ in_b len);
+                        [psimpl; lia|]));
+                    apply noverlap_symmetry,
+                        (noverlap_shrink _ (s5 R_SP ⊖ 32) 32);
+                        [psimpl; lia|];
+                    apply noverlap_symmetry; now destruct NVL]);
+                rewrite MEM;
+                rewrite A0, A1 in H;
+                now repeat (rewrite getmem_noverlap; [|
+                    ((apply (noverlap_shrink _ in_a len);
+                        [psimpl; lia|]) ||
+                    (apply (noverlap_shrink _ in_b len);
+                        [psimpl; lia|]));
+                    apply noverlap_symmetry,
+                        (noverlap_shrink _ (s5 R_SP ⊖ 32) 32);
+                        [psimpl; lia|];
+                    apply noverlap_symmetry; now destruct NVL])
+            | psimpl; apply Answer2; intros a ALen;
+                rewrite A2 in ALen;
+                specialize (H a ALen);
+                rewrite MEM in H;
+                repeat (rewrite getmem_noverlap in H; [|
+                    ((apply (noverlap_shrink _ in_a len);
+                        [psimpl; lia|]) ||
+                    (apply (noverlap_shrink _ in_b len);
+                        [psimpl; lia|]));
+                    apply noverlap_symmetry,
+                        (noverlap_shrink _ (s5 R_SP ⊖ 32) 32);
+                        [psimpl; lia|];
+                    apply noverlap_symmetry; now destruct NVL
+                ]);
+                rewrite A0, A1;
+                now repeat (rewrite getmem_noverlap; [|
+                    ((apply (noverlap_shrink _ in_a len);
+                        [psimpl; lia|]) ||
+                    (apply (noverlap_shrink _ in_b len);
+                        [psimpl; lia|]));
+                    apply noverlap_symmetry,
+                        (noverlap_shrink _ (s5 R_SP ⊖ 32) 32);
+                        [psimpl; lia|];
+                    apply noverlap_symmetry; now destruct NVL])]
+        |]; split; [
+          unfold postcondition;
+          psimpl; rewrite S3, MEM; apply Answer1
+        |]; split; [unfold noverlaps in *; psimpl; 
+          psimpl in NVL; now rewrite SP|];
+          unfold stack; psimpl; rewrite MEM; apply ST).
+    }
+
+    (* To third call *)
+    destruct PRE as (A0 & A1 & A2 & S0 & S1 & S2 & Answer1 & Answer2 & NVL & ST). {
+    step.
+
+    match goal with
+    | [|- context[?x :: ?y :: ?t]] =>
+        change (x :: y :: t) with
+            (x :: nil ++ y :: t)
+    end.
+
+    (* Call CRYPTO_memcmp *)
+    riscv_call crypto_memcmp_correctness;
+        (destruct PRE as (Answer3 & RA & S0' & S1' & S2' & S3 & S4 & SP & MEM);
+        repeat step; unfold postcondition in *; psimpl; split;
+        [rewrite S4, MEM; apply Answer1|]; split;
+        [rewrite S3, MEM; apply Answer2|]; split; [
+            split; intro; [
+                apply Answer3 in H; intros a ALen;
+                rewrite A2 in H;
+                specialize (H a ALen);
+                repeat (rewrite getmem_noverlap in H; [|
+                    ((apply (noverlap_shrink _ in_a len);
+                        [psimpl; lia|]) ||
+                    (apply (noverlap_shrink _ in_b len);
+                        [psimpl; lia|]));
+                    apply noverlap_symmetry,
+                        (noverlap_shrink _ (s5 R_SP ⊖ 32) 32);
+                        [psimpl; lia|];
+                    apply noverlap_symmetry; now destruct NVL]);
+                rewrite MEM;
+                rewrite A0, A1 in H;
+                now repeat (rewrite getmem_noverlap; [|
+                    ((apply (noverlap_shrink _ in_a len);
+                        [psimpl; lia|]) ||
+                    (apply (noverlap_shrink _ in_b len);
+                        [psimpl; lia|]));
+                    apply noverlap_symmetry,
+                        (noverlap_shrink _ (s5 R_SP ⊖ 32) 32);
+                        [psimpl; lia|];
+                    apply noverlap_symmetry; now destruct NVL])
+            | psimpl; apply Answer3; intros a ALen;
+                rewrite A2 in ALen;
+                specialize (H a ALen);
+                rewrite MEM in H;
+                repeat (rewrite getmem_noverlap in H; [|
+                    ((apply (noverlap_shrink _ in_a len);
+                        [psimpl; lia|]) ||
+                    (apply (noverlap_shrink _ in_b len);
+                        [psimpl; lia|]));
+                    apply noverlap_symmetry,
+                        (noverlap_shrink _ (s5 R_SP ⊖ 32) 32);
+                        [psimpl; lia|];
+                    apply noverlap_symmetry; now destruct NVL
+                ]);
+                rewrite A0, A1;
+                now repeat (rewrite getmem_noverlap; [|
+                    ((apply (noverlap_shrink _ in_a len);
+                        [psimpl; lia|]) ||
+                    (apply (noverlap_shrink _ in_b len);
+                        [psimpl; lia|]));
+                    apply noverlap_symmetry,
+                        (noverlap_shrink _ (s5 R_SP ⊖ 32) 32);
+                        [psimpl; lia|];
+                    apply noverlap_symmetry; now destruct NVL])]
+        |]; unfold stack; psimpl; rewrite MEM; apply ST).
+    }
+
+    (* Postcondition *)
+    destruct PRE as (Answer1 & Answer2 & Answer3 & ST).
+    repeat step. unfold stack in ST. split; intro.
+    - unfold postcondition in *.
+      destruct (N.eq_dec (s R_S4) 0),
+               (N.eq_dec (s R_S3) 0),
+               (N.eq_dec (s R_A0) 0);
+        ((now apply Answer1) || (now apply Answer2) || (now apply Answer3) || idtac).
+      repeat (let E := fresh "E" in
+              destruct (N.ltb 0 _) eqn:E in H; [|lia]).
+      psimpl in H. discriminate.
+    - unfold postcondition in *.
+      destruct (N.eq_dec (s R_S4) 0),
+               (N.eq_dec (s R_S3) 0),
+               (N.eq_dec (s R_A0) 0);
+        try rewrite e; try rewrite e0; try rewrite e1; psimpl;
+        auto.
+      apply Answer2 in H. contradiction.
+      apply Answer1 in H. contradiction.
+      apply Answer2 in H. contradiction.
+      apply Answer1 in H. contradiction.
+Qed.
